src/Parsers/NonComputational.v
@@ -80,20 +80,6 @@ Local Open Scope string_like_scope.
 
 Section recursive_descent_parser.
   Context CharType (String : string_like CharType) (G : grammar CharType).
-  Context (T : String -> nonterminal CharType -> Type)
-          (T_reverse_lookup : forall str name, T str (Lookup G name) -> T str [ [ NonTerminal _ name ] ]).
-  Context (parse_pattern_by_picking
-           : forall (parse_pattern_from_split_list
-                     : forall (strs : list String)
-                              (pat : pattern CharType),
-                         ilist (fun sp => T (fst sp) [ [ snd sp ] ]) (combine strs pat))
-                    (str : String)
-                    (pat : pattern CharType),
-               T str [ pat ]).
-  Context (decide_leaf : forall str ch, T str [ [ Terminal ch ] ]).
-  Context (fold_patterns : forall str (pats : list (pattern CharType)),
-                             ilist (fun pat => T str [ pat ]) pats
-                             -> T str pats).
   (** FIXME: The type of the list of nonterminals should be able to
   depend on the string we're parsing, so we can store proofs in it to
   pass down the parse tree to handle impossible cases.  This will
@@ -106,82 +92,134 @@ Section recursive_descent_parser.
           (remove_nonterminal_dec : forall ls nt, is_valid_nonterminal ls nt = true
                                                   -> nonterminal_listT_R (remove_nonterminal ls nt) ls)
           (ntl_wf : well_founded nonterminal_listT_R).
-  Context (make_abort : forall str nt valid_list, is_valid_nonterminal valid_list nt = false -> T str nt).
+  Section generic.
+    Context (T : String -> nonterminal CharType -> Type)
+            (T_reverse_lookup : forall str name, T str (Lookup G name) -> T str [ [ NonTerminal _ name ] ]).
+    Context (parse_pattern_by_picking
+             : forall max_len
+                      (parse_pattern_from_split_list
+                       : forall (strs : list { str : String | Length _ str <= max_len })
+                                (pat : pattern CharType),
+                           ilist (fun sp => T (proj1_sig (fst sp)) [ [ snd sp ] ]) (combine strs pat))
+                      (str : String)
+                      (pf : Length _ str <= max_len)
+                      (pat : pattern CharType),
+                 T str [ pat ]).
+    Context (decide_leaf : forall str ch, T str [ [ Terminal ch ] ]).
+    Context (fold_patterns : forall str (pats : list (pattern CharType)),
+                               ilist (fun pat => T str [ pat ]) pats
+                               -> T str pats).
+    Context (make_abort : forall str nt valid_list, is_valid_nonterminal valid_list nt = false -> T str nt).
 
 
-  Section parts.
-    Section item.
-      Context (str : String)
-              (parse_nonterminal : forall nt, T str nt).
+    Section parts.
+      Section item.
+        Context (str : String)
+                (parse_nonterminal : forall nt, T str nt).
 
-      Definition parse_item it : T str [ [ it ] ]
-        := match it with
-             | Terminal ch => decide_leaf str ch
-             | NonTerminal name => T_reverse_lookup _ (parse_nonterminal (Lookup G name))
-           end.
-    End item.
+        Definition parse_item it : T str [ [ it ] ]
+          := match it with
+               | Terminal ch => decide_leaf str ch
+               | NonTerminal name => T_reverse_lookup _ (parse_nonterminal (Lookup G name))
+             end.
+      End item.
 
-    Section pattern.
-      Variable parse_nonterminal : forall str nt, T str nt.
+      Section pattern.
+        Variable max_len : nat.
+        Variable parse_nonterminal : forall (str : String)
+                                            (pf : Length _ str <= max_len)
+                                            nt, T str nt.
 
-      Definition parse_pattern_from_split_list
-                 (strs : list String)
-                 (pat : pattern CharType)
-      : ilist (fun sp => T (fst sp) [ [ snd sp ] ]) (combine strs pat)
-        := imap_list (fun sp => T (fst sp) [ [ snd sp ] ])
-                     (fun sp => parse_item (parse_nonterminal (fst sp)) (snd sp))
-                     (combine strs pat).
+        Definition parse_pattern_from_split_list
+                   (strs : list { str : String | Length _ str <= max_len })
+                   (pat : pattern CharType)
+        : ilist (fun sp => T (proj1_sig (fst sp)) [ [ snd sp ] ]) (combine strs pat)
+          := imap_list (fun sp => T (proj1_sig (fst sp)) [ [ snd sp ] ])
+                       (fun sp => parse_item (parse_nonterminal _ (proj2_sig (fst sp))) (snd sp))
+                       (combine strs pat).
 
-      Definition parse_pattern (str : String) (pat : pattern CharType) : T str [ pat ]
-        := parse_pattern_by_picking parse_pattern_from_split_list str pat.
-    End pattern.
+        Definition parse_pattern (str : String) (pf : Length _ str <= max_len) (pat : pattern CharType)
+        : T str [ pat ]
+          := parse_pattern_by_picking parse_pattern_from_split_list str pf pat.
+      End pattern.
 
-    Section nonterminal.
-      Section step.
-        Variable parse_nonterminal : forall str nt, T str nt.
+      Section nonterminal.
+        Section step.
+          Variable max_len : nat.
+          Variable parse_nonterminal : forall (str : String)
+                                              (pf : Length _ str <= max_len)
+                                              nt, T str nt.
 
-        Definition parse_nonterminal_step (str : String) (nt : nonterminal CharType) : T str nt
-          := fold_patterns (imap_list (fun pat => T str [ pat ])
-                                      (parse_pattern parse_nonterminal str)
-                                      nt).
-      End step.
+          Definition parse_nonterminal_step (str : String) (pf : Length _ str <= max_len) (nt : nonterminal CharType)
+          : T str nt
+            := fold_patterns (imap_list (fun pat => T str [ pat ])
+                                        (parse_pattern parse_nonterminal str pf)
+                                        nt).
+        End step.
 
-      Section wf.
-        Definition parse_nonterminal_or_abort (valid_list : nonterminal_listT) (max_len : nat)
-                   (str : String)
-                   (pf : Length _ str <= max_len)
-                   (nt : nonterminal CharType)
-        : T str nt.
-        Proof.
-          revert str pf nt.
-          change max_len with (fst (max_len, valid_list)).
-          generalize (max_len, valid_list); clear max_len valid_list.
-          refine (@Fix (nat * nonterminal_listT) _ (well_founded_prod_relation
-                                                      lt_wf
-                                                      ntl_wf)
-                       _ _).
-          intros [max_len valid_list] parse_nonterminal str pf nt.
-          apply le_lt_eq_dec in pf; simpl in *.
-          destruct pf as [pf|pf].
-          { (** [str] got smaller, so we reset the valid nonterminals *)
-            destruct max_len as [|max_len]; [ solve [ destruct (Lt.lt_n_0 _ pf) ] | ].
-            exact (parse_nonterminal
-                     (max_len, initial_nonterminal_data)
-                     (or_introl (Lt.lt_n_Sn _))
-                     str
-                     (le_S_n _ _ pf)
-                     nt). }
-          { (** [str] didn't get smaller, so we cache the fact that we've hit this nonterminal already *)
-            case_eq (is_valid_nonterminal valid_list nt).
-            { (** It was valid, so we can remove it *)
-              intro H.
-              exact (parse_nonterminal
-                       (Length _ str, remove_nonterminal valid_list nt)
-                       (or_intror (conj (eq_sym pf) (remove_nonterminal_dec H)))
-                       str
-                       (reflexivity _)
-                       (** oops, this makes it loop, since we just removed the nt *)
-                       nt). }
-            { (** oops, we already saw this nonterminal in the past.  ABORT! *)
-              apply make_abort. } }
-        Defined.
+        Section wf.
+          Definition parse_nonterminal_or_abort (valid_list : nonterminal_listT) (max_len : nat)
+                     (str : String)
+                     (pf : Length _ str <= max_len)
+                     (nt : nonterminal CharType)
+          : T str nt.
+          Proof.
+            revert str pf nt.
+            change max_len with (fst (max_len, valid_list)).
+            generalize (max_len, valid_list); clear max_len valid_list.
+            refine (@Fix (nat * nonterminal_listT) _ (well_founded_prod_relation
+                                                        lt_wf
+                                                        ntl_wf)
+                         _ _).
+            intros [max_len valid_list] parse_nonterminal str pf nt.
+            apply le_lt_eq_dec in pf; simpl in *.
+            destruct pf as [pf|pf].
+            { (** [str] got smaller, so we reset the valid nonterminals *)
+              destruct max_len as [|max_len]; [ solve [ destruct (Lt.lt_n_0 _ pf) ] | ].
+              specialize (parse_nonterminal
+                            (max_len, initial_nonterminal_data)
+                            (or_introl (Lt.lt_n_Sn _))).
+              apply le_S_n in pf.
+              exact (parse_nonterminal_step parse_nonterminal str pf nt). }
+            { (** [str] didn't get smaller, so we cache the fact that we've hit this nonterminal already *)
+              case_eq (is_valid_nonterminal valid_list nt).
+              { (** It was valid, so we can remove it *)
+                intro H.
+                specialize (parse_nonterminal
+                              (max_len, remove_nonterminal valid_list nt)
+                              (or_intror (conj (reflexivity _) (remove_nonterminal_dec H)))).
+                apply NPeano.Nat.eq_le_incl in pf.
+                exact (parse_nonterminal_step parse_nonterminal str pf nt). }
+              { (** oops, we already saw this nonterminal in the past.  ABORT! *)
+                apply make_abort. } }
+          Defined.
+
+          Definition parse_nonterminal str nt : T str nt
+            := @parse_nonterminal_or_abort initial_nonterminal_data (Length _ str) str
+                                           (NPeano.Nat.eq_le_incl _ _ (reflexivity _)) nt.
+        End wf.
+      End nonterminal.
+    End parts.
+  End generic.
+
+  Section parse_tree.
+    Local Hint Constructors parse_of parse_of_pattern parse_of_item.
+    Local Hint Resolve ParseHead ParsePatternSingleton.
+    Local Hint Extern 1 => apply ParseHead.
+
+    Definition parse_tree_for : forall str nt, option (parse_of String G str nt).
+    Proof.
+      apply (@parse_nonterminal (fun str nt => option (parse_of _ G str nt))).
+      { intros str name [p|]; [ apply Some | exact None ].
+        eauto. }
+      { intros.
+        apply ParsePatternSingleton.
+        constructor.
+        assumption.
+        eapply ParsePatternCons.
+        Print parse_of_pattern.
+      Print parse_of.
+
+End recursive_descent_parser.
+
+Section
